# Schema for database concepts
#
# $Id: db.n3,v 1.12 2006-07-19 21:29:30 timbl Exp $
#
# See http://www.w3.org/DesignIssues/RDB-RDF.html#table
#
#  2006/7 changed daml to owl  timbl

@prefix rdf: <http://www.w3.org/1999/02/22-rdf-syntax-ns#> .
@prefix rdfs: <http://www.w3.org/2000/01/rdf-schema#> .
# @prefix daml: <http://www.daml.org/2001/03/daml+oil#> .
@prefix owl: <http://www.w3.org/2002/07/owl#>.
@prefix log: <http://www.w3.org/2000/10/swap/log#> .
@prefix db: <http://www.w3.org/2000/10/swap/db#> .
@prefix doc: <http://www.w3.org/2000/10/swap/pim/doc#>.
@prefix con: <http://www.w3.org/2000/10/swap/pim/contact#>.
@prefix dc: <http://purl.org/dc/elements/1.1/>.  # @@ no #
@prefix con: <http://www.w3.org/2000/10/swap/pim/contact#>.

<> dc:title "Database terms for the Sematic Web";
   dc:creator [ con:mailbox <mailto:timbl@w3.org>],
              [con:mailbox <mailto:connolly@w3.org>];
   dc:description """
Note that table documents are namespace documents: when you
define a prefix to correspond to the table document's URI with a hash on,
then the table document automatically an RDF schema for the namespace. 
""";
 doc:version "$Id: db.n3,v 1.12 2006-07-19 21:29:30 timbl Exp $".

 
db:Database a rdfs:Class;
    rdfs:label "database";
    rdfs:comment """ """.

db:databaseSchema a rdf:Property;
    rdfs:label "database schema";
    rdfs:comment "The document which describes the form of this database";
    rdfs:domain db:Database;
    rdfs:range db:DatabaseDocument.

db:DatabaseDocument a rdfs:Class;
    rdfs:subClassOf doc:Work;
    rdfs:label "database document";
    rdfs:comment """The resource on the web which describes a database, though not
    the one which contains all the data.
    Convention: Any database <xxx#f> has a databaseDocumemnt <xxx>.""".

db:table a rdf:Property;
    rdfs:label "table";
    rdfs:domain db:Database;
    rdfs:range db:Table;
    rdfs:comment """A table in the database""".

db:Table a rdfs:Class;
    rdfs:subClassOf rdfs:Class;
    rdfs:label "Table";
    rdfs:comment """A Table is a class which has in it a finite
    set of things each of which is described by a row in the database table""".

db:TableDocument a rdfs:Class;
    rdfs:subClassOf doc:Work;
    rdfs:label "table document";
    rdfs:comment """The resource on the web which describes a Table, though not
    the one which contains all the data.
    Convention: Any table <xxx#f> has a tabledocumemnt <xxx>.

   The table document defines a set of db:Column's, one for each column
   of the table.  It is definitive, in that any column in the table MUST
   be described in the table document.

   The table document must also give the database document for the databse the table
   is in.  It is sufficent to quote the URI of the database, as the database document's
   URI follows from the convention.
   This allows a client application to find the other properties of the database.
""".

db:tableSchema a rdf:Property;
    rdfs:label "table schema";
    rdfs:comment "The document which describes the form of this table";
    rdfs:domain db:Table;
    rdfs:range db:TableDocument.

db:tableData a rdf:Property;
    rdfs:label "table data";
    rdfs:comment "The document which gives the data in this table";
    rdfs:domain db:Table;
    rdfs:range doc:Work.

db:Column a rdfs:Class; rdfs:subClassOf rdf:Property;
    rdfs:label "column";
    rdfs:comment """A property corresponding to a database column name.""".

db:column a rdf:Property;
    rdfs:label "column";
    rdfs:domain db:Table; rdfs:range db:Column;
    rdfs:comment """The relationship between a table and one of its columns.

The fact that a table has a db:column in this sense assures that certain conventions
are followed.
1. For any Column <xxx#f> there is always a corresponding table document <xxx>
    which defines it (i.e. says something about it, at least that it is a colmn of the
    table).
""".


db:primaryKeyColumn rdfs:subPropertyOf db:column;
    rdfs:label "primary key column";
    rdfs:comment"""
A primary key column is a column which is either the primary
key, or is one of several columns which form the primary key, of a table.
""".

db:RowDocument a rdfs:Class; rdfs:subClassOf doc:Work;
    rdfs:label "row document";
    rdfs:comment """A row document exists for each row of a table which 
has a primary key.  Its URI is formed by convention by concatenating the
the URI of the table, a slash, and the URI-encoded value of the
primary key value for that row. 

The row document gives the value of each cell in the row.
It identifies the row with a local <#item> URI.
It must also identify <#item> as being of rdf$type of the Table.
""".


#ends
