#   Set Builtins
#
# see cwm_set.py
# 
# $Id: set.n3,v 1.1 2012-01-30 09:30:20 timbl Exp $

@prefix owl: <http://www.w3.org/2002/07/owl#>.

@prefix rdf: <http://www.w3.org/1999/02/22-rdf-syntax-ns#> .
@prefix rdfs: <http://www.w3.org/2000/01/rdf-schema#> .
@prefix doc: <http://www.w3.org/2000/10/swap/pim/doc#>.
@prefix log: <http://www.w3.org/2000/10/swap/log#>.
@prefix set: <http://www.w3.org/2000/10/swap/set#>.
@prefix : <#>.


set:in
    a rdf:Property;
    rdfs:label "in";
    rdfs:comment """This set contains that as a member.
    Cwm will bind the subject to each of the members of the object.""";
    rdfs:range rdfs:Class.
    
set:member
    a rdf:Property;
    owl:inverseOf set:in;
    rdfs:label "member";
    rdfs:comment """This is a member of that set.
    Cwm will bind the object to each of the members of the suject.""";
    rdfs:domain rdfs:Class.

set:union
    a rdf:Property;
    rdfs:range rdfs:Class;
    rdfs:label "union";
    rdfs:comment """The subject is a list [sic] of sets,
    and the objet is the union of the sets in the object""".
    
set:intersection
    a rdf:Property;
    rdfs:range rdfs:Class;
    rdfs:label "intersection";
    rdfs:comment """The subject is a list of sets,
    and the objet is the intersection of the sets in the object""".
    
set:symmetricDifference
    a rdf:Property;
    rdfs:range rdfs:Class;
    rdfs:label "symmetric difference";
    rdfs:comment """The subject is a list of sets,
    and the objet is the symmetricDifference of the sets in the object""".
    
set:difference
    a rdf:Property;
    rdfs:range rdfs:Class;
    rdfs:label "difference";
    rdfs:comment """The subject is a list of sets,
    and the objet is the difference of the sets in the object""".
    
#set:oneOf
#    a rdf:Property;
#    rdfs:range rdfs:Class;
#    rdfs:label "one of";
#    rdfs:comment """The subject @@ in the object""".
    



# ends

